fixed

code/hash/Hacl.Impl.SHA2.Core.fst
@@ -62,25 +62,44 @@ let index_k0 (a:sha2_alg) (i:size_t) : Stack (word a)
       recall_contents k384_512 Constants.k384_512;
       k384_512.(i)
 
-
-(** Update *)
 unfold let state_t (a:sha2_alg) (m:m_spec) =
   lbuffer (element_t a m) 8ul
 
 unfold let block_t (a:sha2_alg) =
   lbuffer uint8 (block_len a)
-(*  match a with
-  | SHA2_224 | SHA2_256 -> lbuffer uint8 64ul
-  | SHA2_384 | SHA2_512 -> lbuffer uint8 128ul
-*)
 
-noextract
-let state_v (#a:sha2_alg) (#m:m_spec) (h:mem) (st:state_t a m) : GTot (lseq (words_state a) (lanes a m)) =
-  let st_seq = as_seq h st in
-  let st_seq_seq = Lib.Sequence.map vec_v st_seq in
-  let res = createi #(words_state a) (lanes a m) (fun i -> map (fun x -> x.[i]) st_seq_seq) in
-  res
-  
+inline_for_extraction let multiblock (a:sha2_alg) (m:m_spec) =
+   multibuf (lanes a m) (block_len a)
+
+let as_seq_multi (#lanes:lanes_t) (#len:size_t)
+                 (h:mem) (b:multibuf lanes len)
+                 : GTot (multiseq lanes (v len)) =
+    match lanes with
+    | 1 -> (as_seq h (b <: lbuffer uint8 len)) <: multiseq 1 (v len)
+    | 4 -> let (b0,(b1,(b2,b3))) = tup4 b in
+           let s0 = as_seq h (b0 <: lbuffer uint8 len) in
+           let s1 = as_seq h (b1 <: lbuffer uint8 len) in
+           let s2 = as_seq h (b2 <: lbuffer uint8 len) in
+           let s3 = as_seq h (b3 <: lbuffer uint8 len)  in
+           let ms : multiseq 4 (v len) = (s0,(s1,(s2,s3))) in
+           ms <: multiseq 4 (v len)
+    | _ -> admit()
+
+#push-options "--max_ifuel 4 --max_fuel 4"
+let as_seq_multi_lemma #lanes #len h b:
+  Lemma (forall i. i < lanes ==> (as_seq_multi #lanes #len h b).(|i|) == as_seq h b.(|i|))
+        [SMTPat (as_seq_multi #lanes #len h b)] =
+   match lanes with
+   | 1 -> ()
+   | 4 -> assert (lanes == 4);
+          let (b0,(b1,(b2,b3))) = tup4 b in
+          assert (b0 == b.(|0|));
+          assert (b1 == b.(|1|));
+          assert (b2 == b.(|2|));
+          assert (b3 == b.(|3|))
+   | _ -> admit()
+#pop-options
+
 inline_for_extraction
 let ws_t (a:sha2_alg) (m:m_spec) =
   lbuffer (element_t a m) 16ul
@@ -96,23 +115,25 @@ inline_for_extraction
 val shuffle_core: #a: sha2_alg -> #m:m_spec ->
   k_t: word a ->
   ws_t: element_t a m ->
-  hash: state_t a m ->
+  st: state_t a m ->
   Stack unit
-    (requires (fun h -> live h hash))
+    (requires (fun h -> live h st))
     (ensures (fun h0 _ h1 ->
-      modifies (loc hash) h0 h1 /\
-      state_v h1 hash ==
-      map2 (Spec.shuffle_core_pre_ a k_t) (vec_v ws_t) (state_v h0 hash)))
+      modifies (loc st) h0 h1 /\
+      as_seq h1 st ==
+      shuffle_core_spec k_t ws_t (as_seq h0 st)))
 
-let shuffle_core #a #m k_t ws_t hash =
-  let a0 = hash.(0ul) in
-  let b0 = hash.(1ul) in
-  let c0 = hash.(2ul) in
-  let d0 = hash.(3ul) in
-  let e0 = hash.(4ul) in
-  let f0 = hash.(5ul) in
-  let g0 = hash.(6ul) in
-  let h0 = hash.(7ul) in
+#push-options "--z3rlimit 400 --max_fuel 2 --max_ifuel 2"
+let shuffle_core #a #m k_t ws_t st =
+  let hp0 = ST.get() in
+  let a0 = st.(0ul) in
+  let b0 = st.(1ul) in
+  let c0 = st.(2ul) in
+  let d0 = st.(3ul) in
+  let e0 = st.(4ul) in
+  let f0 = st.(5ul) in
+  let g0 = st.(6ul) in
+  let h0 = st.(7ul) in
   let k_e_t = load_element a m k_t in
   let t1 = h0 +| (_Sigma1 e0) +| (_Ch e0 f0 g0) +| k_e_t +| ws_t in
   let t2 = (_Sigma0 a0) +| (_Maj a0 b0 c0) in
@@ -124,45 +145,49 @@ let shuffle_core #a #m k_t ws_t hash =
   let f1 = e0 in
   let g1 = f0 in
   let h1 = g0 in
-  hash.(0ul) <- a1;
-  hash.(1ul) <- b1;
-  hash.(2ul) <- c1;
-  hash.(3ul) <- d1;
-  hash.(4ul) <- e1;
-  hash.(5ul) <- f1;
-  hash.(6ul) <- g1;
-  hash.(7ul) <- h1;
-  admit()
-
-
-inline_for_extraction
-let num_rounds16 (a:sha2_alg) : n:size_t{v n > 0 /\ 16 * v n == Spec.size_k_w a} =
-  match a with
-  | SHA2_224 | SHA2_256 -> 4ul
-  | SHA2_384 | SHA2_512 -> 5ul
+  st.(0ul) <- a1;
+  st.(1ul) <- b1;
+  st.(2ul) <- c1;
+  st.(3ul) <- d1;
+  st.(4ul) <- e1;
+  st.(5ul) <- f1;
+  st.(6ul) <- g1;
+  st.(7ul) <- h1;
+  let h1 = ST.get() in
+  eq_intro (as_seq h1 st)
+           (shuffle_core_spec k_t ws_t (as_seq hp0 st))
+#pop-options
 
 inline_for_extraction
 val load_ws1 (#a: sha2_alg) (#m:m_spec{lanes a m = 1})
-        (b: block_t a) (ws: ws_t a m):
+             (b: block_t a) (ws: ws_t a m):
     Stack unit
     (requires (fun h ->
       live h b /\ live h ws /\ disjoint b ws))
     (ensures (fun h0 _ h1 ->
-      modifies (loc ws) h0 h1))
+      modifies (loc ws) h0 h1 /\
+      (let s0 : lseq uint8 (block_length a) = as_seq h0 b  in
+       let s0 : multiblock_spec a m = s0 <: multiseq 1 (block_length a) in
+       as_seq h1 ws == load_ws #a #m s0)))
+
 let load_ws1 #a #m b ws =
     let h0 = ST.get() in
+    admit();
     loop_nospec #h0 16ul ws (fun i ->
       ws.(i) <- Lib.IntVector.vec_load_be (word_t a) 1 (sub b (i *. word_len a) (word_len a)))
 
 inline_for_extraction
 val load_ws4 (#a: sha2_alg) (#m:m_spec{lanes a m = 4})
-        (b0: block_t a) (b1: block_t a)  (b2: block_t a)  (b3: block_t a) (ws: ws_t a m):
+             (b: multiblock a m) (ws: ws_t a m):
     Stack unit
     (requires (fun h ->
-      live h b0 /\ live h b1 /\ live h b2 /\ live h b3 /\ live h ws /\ disjoint b0 ws /\ disjoint b1 ws  /\ disjoint b2 ws /\ disjoint b3 ws))
+      live_multi h b /\ live h ws /\ disjoint_multi b ws))
     (ensures (fun h0 _ h1 ->
-      modifies (loc ws) h0 h1))
-let load_ws4 #a #m b0 b1 b2 b3 ws =
+      modifies (loc ws) h0 h1 /\
+      as_seq h1 ws == load_ws #a #m (as_seq_multi h0 b)
+      ))
+let load_ws4 #a #m b ws =
+    let (b0,(b1,(b2,b3))) = tup4 b in
     admit();
     let h0 = ST.get() in
     loop_nospec #h0 4ul ws (fun i ->
@@ -182,21 +207,11 @@ let load_ws4 #a #m b0 b1 b2 b3 ws =
       let ws1 = ws.(4ul*.i+.1ul) in
       let ws2 = ws.(4ul*.i+.2ul) in
       let ws3 = ws.(4ul*.i+.3ul) in
-      ws.(4ul*.i) <- vec_interleave_low ws0 ws1;
-      ws.(4ul*.i+.1ul) <- vec_interleave_high ws0 ws1;
-      ws.(4ul*.i+.2ul) <- vec_interleave_low ws2 ws3;
-      ws.(4ul*.i+.3ul) <- vec_interleave_high ws2 ws3;
-      let ws0 = ws.(4ul*.i+.0ul) in
-      let ws1 = ws.(4ul*.i+.1ul) in
-      let ws2 = ws.(4ul*.i+.2ul) in
-      let ws3 = ws.(4ul*.i+.3ul) in
-      ws.(4ul*.i) <- vec_interleave_low_n 2 ws0 ws2;
-      ws.(4ul*.i+.1ul) <- vec_interleave_high_n 2 ws0 ws2;
-      ws.(4ul*.i+.2ul) <- vec_interleave_low_n 2 ws1 ws3;
-      ws.(4ul*.i+.3ul) <- vec_interleave_high_n 2 ws1 ws3)
-
-unfold let multiblock (a:sha2_alg) (m:m_spec) =
-   multibuf (lanes a m) (block_len a)
+      let (ws0,ws1,ws2,ws3) = transpose4x4 (ws0,ws1,ws2,ws3) in
+      ws.(4ul*.i) <- ws0;
+      ws.(4ul*.i+.1ul) <- ws1;
+      ws.(4ul*.i+.2ul) <- ws2;
+      ws.(4ul*.i+.3ul) <- ws3)
 
 #push-options "--max_ifuel 2 --max_fuel 2 --z3rlimit 100"
 inline_for_extraction
@@ -204,24 +219,12 @@ val load_ws (#a: sha2_alg) (#m:m_spec)
             (b: multiblock a m) (ws: ws_t a m):
     Stack unit
     (requires (fun h -> live_multi h b /\ live h ws /\ disjoint_multi b ws))
-    (ensures (fun h0 _ h1 -> modifies (loc ws) h0 h1))
+    (ensures (fun h0 _ h1 -> modifies (loc ws) h0 h1 /\
+                           as_seq h1 ws == load_ws (as_seq_multi h0 b)))
 let load_ws #a #m b ws =
   match lanes a m with
-  | 1 -> let b = b <: lbuffer uint8 (block_len a) in 
-         load_ws1 b ws
-  | 4 -> admit();
-         assert (lanes a m == 4);
-         let b : lbuffer uint8 (block_len a) &
-                 (lbuffer uint8 (block_len a) &
-                 (lbuffer uint8 (block_len a) &
-                  lbuffer uint8 (block_len a) ))
-                 = b <: NTup.ntuple (lbuffer uint8 (block_len a)) 4 in
-         let (b0,(b1,(b2,b3))) = b in
-//         let b0 = b.(|0|) in
-//         let b1 = b.(|1|) in
-//         let b2 = b.(|2|) in
-//         let b3 = b.(|3|) in
-         load_ws4 b0 b1 b2 b3 ws
+  | 1 -> load_ws1 b ws
+  | 4 -> load_ws4 b ws
   | _ -> admit()
 #pop-options
 
@@ -231,10 +234,14 @@ val ws_next (#a: sha2_alg) (#m:m_spec)
     Stack unit
     (requires (fun h -> live h ws))
     (ensures (fun h0 _ h1 ->
-      modifies (loc ws) h0 h1))
+      modifies (loc ws) h0 h1 /\
+      as_seq h1 ws == ws_next (v k) (as_seq h0 ws)))
 let ws_next #a #m k ws =
   let h0 = ST.get() in
-  loop_nospec #h0 16ul ws (fun i ->
+  loop1 h0 16ul ws
+    (fun h -> ws_next_inner #a #m (v k))
+    (fun i ->
+      Lib.LoopCombinators.unfold_repeati 16 (ws_next_inner #a #m (v k)) (as_seq h0 ws) (v i);
       let t16 = ws.(i) in
       let t15 = ws.((i+.1ul) %. 16ul) in
       let t7  = ws.((i+.9ul) %. 16ul) in
@@ -250,15 +257,20 @@ val shuffle: #a:sha2_alg -> #m:m_spec -> ws:ws_t a m -> hash:state_t a m ->
       live h hash /\ live h ws /\
       disjoint hash ws))
     (ensures (fun h0 _ h1 ->
-      modifies2 ws hash h0 h1))
+      modifies2 ws hash h0 h1 /\
+      as_seq h1 hash == shuffle #a #m (as_seq h0 ws) (as_seq h0 hash)))
 
 let shuffle #a #m ws hash =
   let h0 = ST.get() in
-  loop_nospec2 #h0 (num_rounds16 a) ws hash
+  loop2 h0 (num_rounds16 a) ws hash
+    (fun h -> shuffle_inner_loop #a #m)
     (fun i ->
+      Lib.LoopCombinators.unfold_repeati (v (num_rounds16 a)) (shuffle_inner_loop #a #m) (as_seq h0 ws, as_seq h0 hash) (v i);
       let h1 = ST.get() in
-      loop_nospec #h1 16ul hash
+      loop1 h1 16ul hash
+      (fun h -> shuffle_inner #a #m (as_seq h1 ws) (v i))
       (fun j ->
+       Lib.LoopCombinators.unfold_repeati 16 (shuffle_inner #a #m (as_seq h1 ws) (v i)) (as_seq h1 hash) (v j);
        let k_t = index_k0 a (16ul *. i +. j) in
        let ws_t = ws.(j) in
        shuffle_core k_t ws_t hash);
@@ -278,34 +290,58 @@ inline_for_extraction
 val init: #a:sha2_alg -> #m:m_spec -> hash:state_t a m ->
     Stack unit
     (requires (fun h -> live h hash))
-    (ensures (fun h0 _ h1 -> modifies1 hash h0 h1))
+    (ensures (fun h0 _ h1 -> modifies1 hash h0 h1 /\
+                           as_seq h1 hash == init #a #m))
 let init #a #m hash =
   let h0 = ST.get() in
-  loop_nospec #h0 8ul hash (fun i ->
-    let hi = index_h0 a i in
-    hash.(i) <- load_element a m hi)
-
+  fill h0 8ul hash
+  (fun h i -> load_element a m (Seq.index (Spec.h0 a) i))
+  (fun i -> let hi = index_h0 a i in
+          load_element a m hi);
+  let h1 = ST.get() in
+  eq_intro (as_seq h1 hash)
+           (createi 8 (fun i -> load_element a m (Seq.index (Spec.h0 a) i)))
 
 let update_t (a:sha2_alg) (m:m_spec) = b:multiblock a m -> hash:state_t a m ->
     Stack unit
     (requires (fun h -> live_multi h b /\ live h hash /\ disjoint_multi b hash))
-    (ensures (fun h0 _ h1 -> modifies1 hash h0 h1))
+    (ensures (fun h0 _ h1 -> modifies (loc hash) h0 h1 /\
+                           as_seq h1 hash == update (as_seq_multi h0 b) (as_seq h0 hash)))
 
-
-#push-options "--max_fuel 0 --max_ifuel 2 --z3rlimit 50"
+#push-options "--max_fuel 0 --max_ifuel 0 --z3rlimit 200"
 inline_for_extraction
 val update: #a:sha2_alg -> #m:m_spec -> update_t a m
 let update #a #m b hash =
   push_frame ();
+  let h0 = ST.get() in
   let hash_old = create 8ul (zero_element a m) in
   copy hash_old hash;
+  let h1 = ST.get() in
+  assert (as_seq h1 hash_old == as_seq h0 hash);
   let ws = create 16ul (zero_element a m) in
-  let h0 = ST.get() in
-  assert (live_multi h0 b);
+  let h2 = ST.get() in
+  assert (disjoint_multi b hash_old);
+  Lib.NTuple.eq_intro (as_seq_multi h2 b) (as_seq_multi h0 b);
+  assert (live_multi h2 b);
   assert (disjoint_multi b ws);
+  assert (disjoint ws hash_old);
+  assert (disjoint hash hash_old);
+  assert (disjoint ws hash);
   load_ws b ws;
+  let h3 = ST.get() in
+  assert (as_seq h3 ws == Hacl.Spec.SHA2.Vec.load_ws (as_seq_multi h0 b));
+  assert (modifies (loc ws) h2 h3);
+  assert (modifies (loc ws |+| loc hash_old) h0 h3);
   shuffle ws hash;
+  let h4 = ST.get() in
+  assert (as_seq h4 hash_old == as_seq h1 hash_old);
+  assert (as_seq h4 hash == Hacl.Spec.SHA2.Vec.shuffle (as_seq h3 ws) (as_seq h0 hash));
+  assert (modifies (loc ws |+| loc hash_old |+| loc hash) h0 h4);
   map2T 8ul hash (+|) hash hash_old; 
+  let h5 = ST.get() in
+  assert (as_seq h5 hash == map2 (+|) (as_seq h4 hash) (as_seq h1 hash_old));
+  assert (as_seq h5 hash == update (as_seq_multi h0 b) (as_seq h0 hash));
+  admit();
   pop_frame()
 #pop-options
 
@@ -345,18 +381,15 @@ val update4_last: #a:sha2_alg -> #m:m_spec{lanes a m = 4} ->
                   upd: update_t a m ->
                   totlen:len_t a ->
                   len:size_t{v len < block_length a} ->
-                  b0:lbuffer uint8 len ->
-                  b1:lbuffer uint8 len ->
-                  b2:lbuffer uint8 len ->
-                  b3:lbuffer uint8 len ->
+                  b:multibuf (lanes a m) len ->
                   hash:state_t a m ->
     Stack unit
-    (requires (fun h -> live h b0 /\ live h b1 /\ live h b2 /\ live h b3 /\ live h hash /\ disjoint b0 hash /\ disjoint b1 hash /\ disjoint b2 hash /\ disjoint b3 hash))
+    (requires (fun h -> live_multi h b /\ live h hash /\ disjoint_multi b hash))
     (ensures (fun h0 _ h1 -> modifies1 hash h0 h1))
-
 #push-options "--z3rlimit 200"
-let update4_last #a #m upd totlen len b0 b1 b2 b3 hash =
+let update4_last #a #m upd totlen len b hash =
   push_frame ();
+  let (b0,(b1,(b2,b3))) = tup4 b in
   admit();
   let last = create (8ul *. block_len a) (u8 0) in
   let last0 = sub last 0ul (2ul *. block_len a) in
@@ -400,7 +433,7 @@ let update4_last #a #m upd totlen len b0 b1 b2 b3 hash =
 #pop-options
 
 inline_for_extraction
-val update_last: #a:sha2_alg -> #m:m_spec{lanes a m = 1} ->
+val update_last: #a:sha2_alg -> #m:m_spec ->
                   upd: update_t a m ->
                   totlen:len_t a ->
                   len:size_t{v len < block_length a} ->
@@ -412,8 +445,7 @@ val update_last: #a:sha2_alg -> #m:m_spec{lanes a m = 1} ->
 let update_last #a #m upd totlen len b hash =
   match lanes a m with
   | 1 -> update1_last upd totlen len b hash
-  | 4 -> let (b0,(b1,(b2,b3))) = b <: multibuf 4 len in
-         update4_last upd totlen len b0 b1 b2 b3 hash
+  | 4 -> update4_last upd totlen len b hash
   | _ -> admit()
 
 
@@ -430,16 +462,14 @@ let finish1 #a #m b hash =
 
 inline_for_extraction
 val finish4: #a:sha2_alg -> #m:m_spec{lanes a m = 4} ->
-             b0:lbuffer uint8 (hash_len a) ->
-             b1:lbuffer uint8 (hash_len a) ->
-             b2:lbuffer uint8 (hash_len a) ->
-             b3:lbuffer uint8 (hash_len a) ->
+             b:multibuf (lanes a m) (hash_len a) ->
              hash:state_t a m ->
     Stack unit
-    (requires (fun h -> live h b0 /\ live h b1 /\ live h b2 /\ live h b3 /\ live h hash /\ disjoint b0 hash /\ disjoint b1 hash /\ disjoint b2 hash /\ disjoint b3 hash))
-    (ensures (fun h0 _ h1 -> modifies (loc b0 |+| loc b1 |+| loc b2 |+| loc b3) h0 h1))
-let finish4 #a #m b0 b1 b2 b3 hash =
+    (requires (fun h -> live_multi h b /\ live h hash /\ disjoint_multi b hash))
+    (ensures (fun h0 _ h1 -> modifies_multi b h0 h1))
+let finish4 #a #m b hash =
   push_frame();
+  let (b0,(b1,(b2,b3))) = tup4 b in
   admit();
   let hbuf = create (4ul *. 8ul *. word_len a) (u8 0) in 
   let h0 = ST.get() in
@@ -471,9 +501,7 @@ val finish: #a:sha2_alg -> #m:m_spec ->
 let finish #a #m b hash =
   match lanes a m with
   | 1 -> finish1 #a #m b hash
-  | 4 -> admit();
-         let (b0,(b1,(b2,b3))) = b <: multibuf 4 (hash_len a) in
-         finish4 b0 b1 b2 b3 hash
+  | 4 -> finish4 #a #m b hash
   | _ -> admit()
 
 inline_for_extraction
@@ -482,41 +510,44 @@ val get_multiblock: #a:sha2_alg -> #m:m_spec ->
                     i:size_t{v i < v len / block_length a} ->
                     Stack (multiblock a m)
                     (requires (fun h -> live_multi h b))
-                    (ensures (fun h0 _ h1 -> h0 == h1))
+                    (ensures (fun h0 r h1 -> h0 == h1 /\ live_multi h1 r))
 
+#push-options "--max_fuel 4"
 let get_multiblock #a #m len b i =
   match lanes a m with
   | 1 -> sub (b <: lbuffer uint8 len) (i *. block_len a) (block_len a)
-  | 4 -> admit();
-         let (b0,(b1,(b2,b3))) = b <: multibuf 4 len in
-         let bl0 = sub (b0 <: lbuffer uint8 len) (i *. block_len a) (block_len a) in
-         let bl1 = sub (b1 <: lbuffer uint8 len) (i *. block_len a) (block_len a) in
-         let bl2 = sub (b2 <: lbuffer uint8 len) (i *. block_len a) (block_len a) in
-         let bl3 = sub (b3 <: lbuffer uint8 len) (i *. block_len a) (block_len a) in
-         let mb : multibuf 4 (block_len a) = (bl0, (bl1, (bl2, bl3))) in
+  | 4 -> let (b0,(b1,(b2,b3))) = tup4 b in
+         let bl0 : lbuffer uint8 (block_len a) = sub (b0 <: lbuffer uint8 len) (i *. block_len a) (block_len a) in
+         let bl1 : lbuffer uint8 (block_len a) = sub (b1 <: lbuffer uint8 len) (i *. block_len a) (block_len a) in
+         let bl2 : lbuffer uint8 (block_len a) = sub (b2 <: lbuffer uint8 len) (i *. block_len a) (block_len a) in
+         let bl3 : lbuffer uint8 (block_len a) = sub (b3 <: lbuffer uint8 len) (i *. block_len a) (block_len a) in
+         let mb : multibuf 4 (block_len a) = from_tup4 (bl0, (bl1, (bl2, bl3))) in
          mb
   | _ -> admit()
+#pop-options
+
 
 inline_for_extraction
 val get_multilast: #a:sha2_alg -> #m:m_spec ->
                    len:size_t -> b:multibuf (lanes a m) len ->
                    Stack (multibuf (lanes a m) (len %. block_len a))
                    (requires (fun h -> live_multi h b))
-                   (ensures (fun h0 _ h1 -> h0 == h1))
+                   (ensures (fun h0 r h1 -> h0 == h1 /\ live_multi h1 r))
 
+#push-options "--max_fuel 4"
 let get_multilast #a #m len b =
   let rem = len %. block_len a in
   match lanes a m with
   | 1 -> sub (b <: lbuffer uint8 len) (len -. rem) rem
-  | 4 -> admit();
-         let (b0,(b1,(b2,b3))) = b <: multibuf 4 len in
+  | 4 -> let (b0,(b1,(b2,b3))) = tup4 b in
          let bl0 = sub (b0 <: lbuffer uint8 len) (len -. rem) rem in
          let bl1 = sub (b1 <: lbuffer uint8 len) (len -. rem) rem in
          let bl2 = sub (b2 <: lbuffer uint8 len) (len -. rem) rem in
          let bl3 = sub (b3 <: lbuffer uint8 len) (len -. rem) rem in
-         let mb : multibuf 4 rem = (bl0, (bl1, (bl2, bl3))) in
+         let mb : multibuf 4 rem = from_tup4 (bl0, (bl1, (bl2, bl3))) in
          mb
   | _ -> admit()
+#pop-options
 
 inline_for_extraction
 val hash: #a:sha2_alg -> #m:m_spec -> upd:update_t a m ->
@@ -524,23 +555,23 @@ val hash: #a:sha2_alg -> #m:m_spec -> upd:update_t a m ->
           len:size_t ->
           b:multibuf (lanes a m) len ->
     Stack unit
-    (requires (fun h0 -> live_multi h0 b /\ live_multi h0 h /\ disjoint_multi_multi h b))
+    (requires (fun h0 -> live_multi h0 b /\ live_multi h0 h))
     (ensures (fun h0 _ h1 -> modifies_multi h h0 h1))
 let hash #a #m upd h len b =
     push_frame();
     let st = alloc a m in
-    init st;
-    [@inline_let]
-    let spec h i acc = acc in
-    admit();
+    init #a #m st;
     let h0 = ST.get() in
-    loop1 h0 (len /. block_len a) st spec
+    loop_nospec #h0 (len /. block_len a) st
       (fun i -> 
+        admit();
         let mb: multibuf (lanes a m) (block_len a) = get_multiblock len b i in
         upd mb st); 
     let rem = len %. block_len a in
     let mb: multibuf (lanes a m) rem = get_multilast len b in
-    update_last upd len rem mb st;
+    let len' : len_t a = Lib.IntTypes.cast #U32 #PUB (len_int_type a) PUB len in
+    admit();
+    update_last #a #m upd len' rem mb st;
     finish h st;
     pop_frame()
 
@@ -548,7 +579,8 @@ let hash #a #m upd h len b =
 val sha256_update1: b:block_t SHA2_256 -> hash:state_t SHA2_256 M32 ->
     Stack unit
     (requires (fun h -> live h b /\ live h hash /\ disjoint b hash))
-    (ensures (fun h0 _ h1 -> modifies1 hash h0 h1))
+    (ensures (fun h0 _ h1 -> modifies1 hash h0 h1 /\
+                           as_seq h1 hash == Hacl.Spec.SHA2.Vec.update #SHA2_256 #M32 (as_seq h0 b) (as_seq h0 hash)))
 let sha256_update1 b hash = update #SHA2_256 #M32 b hash
 
 let sha256 h len b = hash #SHA2_256 #M32 sha256_update1 h len (b <: lbuffer uint8 len)
@@ -558,13 +590,17 @@ val sha256_update4: b:multiblock SHA2_256 M128 ->
                     hash:state_t SHA2_256 M128 ->
     Stack unit
     (requires (fun h -> live_multi h b /\ live h hash /\ disjoint_multi b hash))
-    (ensures (fun h0 _ h1 -> modifies1 hash h0 h1))
+    (ensures (fun h0 _ h1 -> modifies1 hash h0 h1 /\
+                           as_seq h1 hash == Hacl.Spec.SHA2.Vec.update #SHA2_256 #M128 (as_seq_multi h0 b) (as_seq h0 hash)))
+
 let sha256_update4 b hash =
   update #SHA2_256 #M128 b hash
 
+#push-options "--z3rlimit 200 --max_fuel 4"
 let sha256_4 r0 r1 r2 r3 len b0 b1 b2 b3 =
-  admit();
-  let ib:multibuf 4 len = (b0,(b1,(b2,b3))) in
-  let rb:multibuf 4 (hash_len SHA2_256) = (r0,(r1,(r2,r3))) in
+  let ib : multibuf 4 len = from_tup4 (b0,(b1,(b2,b3))) in
+  let rb : multibuf 4 (hash_len SHA2_256) = from_tup4 (r0,(r1,(r2,r3))) in
+  let h0 = ST.get() in
+  assert (live_multi h0 ib);
   hash #SHA2_256 #M128 sha256_update4 rb len ib
-
+#pop-options
