code/hash/Hacl.Spec.SHA2.Vec.fst
@@ -2,10 +2,10 @@ module Hacl.Spec.SHA2.Vec
 
 open FStar.Mul
 open Lib.IntTypes
+open Lib.NTuple
 open Lib.Sequence
-open Lib.Buffer
 open Lib.IntVector
-module NTup = Lib.NTuple
+open Lib.LoopCombinators
 open Spec.Hash.Definitions
 module Constants = Spec.SHA2.Constants
 module Spec = Spec.SHA2
@@ -147,7 +147,380 @@ let _sigma1_lemma #a #m x :
          Lib.Sequence.map (Spec._sigma1 a) (vec_v x)) =
         Lib.Sequence.eq_intro (vec_v (_sigma1 #a #m x)) (Lib.Sequence.map (Spec._sigma1 a) (vec_v x))
 
+noextract
+let state_spec (a:sha2_alg) (m:m_spec) =
+  lseq (element_t a m) 8
+
+noextract
+let block_spec (a:sha2_alg) =
+  lseq uint8 (block_length a)
+noextract
+let ws_spec (a:sha2_alg) (m:m_spec) =
+  lseq (element_t a m) 16
+
+noextract
+let state_v (#a:sha2_alg) (#m:m_spec) (st:state_spec a m) : GTot (lseq (words_state a) (lanes a m)) =
+  let st_seq_seq = Lib.Sequence.map vec_v st in
+  let res = createi #(words_state a) (lanes a m) (fun i -> map (fun x -> x.[i]) st_seq_seq) in
+  res
+
+noextract
+let ws_v (#a:sha2_alg) (#m:m_spec) (st:ws_spec a m) : GTot (lseq (lseq (word a) 16) (lanes a m)) =
+  let st_seq_seq = Lib.Sequence.map vec_v st in
+  let res = createi #(lseq (word a) 16) (lanes a m) (fun i -> map (fun x -> x.[i]) st_seq_seq) in
+  res
+
+noextract
+val shuffle_core_spec: #a: sha2_alg -> #m:m_spec ->
+                       k_t: word a ->
+                       ws_t: element_t a m ->
+                       st: state_spec a m ->
+                       state_spec a m
+let shuffle_core_spec #a #m k_t ws_t st =
+  let a0 = st.[0] in
+  let b0 = st.[1] in
+  let c0 = st.[2] in
+  let d0 = st.[3] in
+  let e0 = st.[4] in
+  let f0 = st.[5] in
+  let g0 = st.[6] in
+  let h0 = st.[7] in
+  let k_e_t = load_element a m k_t in
+  let t1 = h0 +| (_Sigma1 e0) +| (_Ch e0 f0 g0) +| k_e_t +| ws_t in
+  let t2 = (_Sigma0 a0) +| (_Maj a0 b0 c0) in
+  let a1 = t1 +| t2 in
+  let b1 = a0 in
+  let c1 = b0 in
+  let d1 = c0 in
+  let e1 = d0 +| t1 in
+  let f1 = e0 in
+  let g1 = f0 in
+  let h1 = g0 in
+  create8 a1 b1 c1 d1 e1 f1 g1 h1
 
 
+inline_for_extraction
+let num_rounds16 (a:sha2_alg) : n:size_t{v n > 0 /\ 16 * v n == Spec.size_k_w a} =
+  match a with
+  | SHA2_224 | SHA2_256 -> 4ul
+  | SHA2_384 | SHA2_512 -> 5ul
+
+noextract
+let multiseq (lanes:lanes_t) (len:size_nat) =
+  ntuple (lseq uint8 len) lanes
+
+inline_for_extraction
+let tup4 #a (#l:lanes_t{l = 4}) (t:ntuple a l) : a & (a & (a & a)) =
+  assert (ntuple a l == ntuple a 4);
+  t <: ntuple a 4
+
+inline_for_extraction
+let from_tup4 #a (#l:lanes_t{l = 4}) (t:a & (a & (a & a))) : ntuple a l =
+  assert (ntuple a l == ntuple a 4);
+  t <: ntuple a 4
+
+noextract
+let multiblock_spec (a:sha2_alg) (m:m_spec) =
+  multiseq (lanes a m) (block_length a)
+
+#push-options "--z3rlimit 100"
+noextract
+let load_blocks (#a:sha2_alg) (#m:m_spec) (b:multiblock_spec a m) : ws_spec a m =
+  let l = lanes a m in
+  createi 16 (fun i ->
+                    let idx_i = i % l in
+                    let idx_j = i / l in
+                    vec_from_bytes_be (word_t a) l (sub b.(|idx_i|) (idx_j * l * word_length a) (l * word_length a)))
+#pop-options
+
+noextract
+let transpose_ws1 (#a:sha2_alg) (#m:m_spec{lanes a m == 1}) (ws:ws_spec a m) : ws_spec a m = ws
+
+inline_for_extraction
+let transpose4x4 #vt
+                 (vs : (vec_t vt 4 & vec_t vt 4 & vec_t vt 4 & vec_t vt 4)) :
+                       (vec_t vt 4 & vec_t vt 4 & vec_t vt 4 & vec_t vt 4) =
+    let (v0,v1,v2,v3) = vs in
+    let v0' = vec_interleave_low v0 v1 in
+    let v1' = vec_interleave_high v0 v1 in
+    let v2' = vec_interleave_low v2 v3 in
+    let v3' = vec_interleave_high v2 v3 in
+    let v0'' = vec_interleave_low_n 2 v0' v2' in
+    let v1'' = vec_interleave_high_n 2 v0' v2' in
+    let v2'' = vec_interleave_low_n 2 v1' v3' in
+    let v3'' = vec_interleave_high_n 2 v1' v3' in
+    (v0'',v1'',v2'',v3'')
+
+noextract
+let transpose_ws4 (#a:sha2_alg) (#m:m_spec{lanes a m == 4}) (ws:ws_spec a m) : ws_spec a m =
+    let (ws0,ws1,ws2,ws3) = transpose4x4 (ws.[0], ws.[1], ws.[2], ws.[3]) in
+    let (ws4,ws5,ws6,ws7) = transpose4x4 (ws.[4], ws.[5], ws.[6], ws.[7]) in
+    let (ws8,ws9,ws10,ws11) = transpose4x4 (ws.[8], ws.[9], ws.[10], ws.[11]) in
+    let (ws12,ws13,ws14,ws15) = transpose4x4 (ws.[12], ws.[13], ws.[14], ws.[15]) in
+    create16 ws0 ws1 ws2 ws3 ws4 ws5 ws6 ws7 ws8 ws9 ws10 ws11 ws12 ws13 ws14 ws15
+    
+noextract
+let transpose_ws (#a:sha2_alg) (#m:m_spec) (ws:ws_spec a m) : ws_spec a m =
+  match lanes a m with
+  | 1 -> transpose_ws1 #a #m ws
+  | 4 -> transpose_ws4 #a #m ws
+  | _ -> admit()
 
 
+noextract
+let load_ws (#a:sha2_alg) (#m:m_spec) (b:multiblock_spec a m) : ws_spec a m =
+  let ws = load_blocks #a #m b in
+  transpose_ws #a #m ws
+
+noextract
+let ws_next_inner (#a:sha2_alg) (#m:m_spec)
+                  (k:size_nat{k > 0 /\ k < v (num_rounds16 a)})
+                  (i:size_nat{i < 16})
+                  (ws:ws_spec a m) : ws_spec a m =
+      let t16 = ws.[i] in
+      let t15 = ws.[(i+1) % 16] in
+      let t7  = ws.[(i+9) % 16] in
+      let t2  = ws.[(i+14) % 16] in
+      let s1 = _sigma1 t2 in
+      let s0 = _sigma0 t15 in
+      ws.[i] <- (s1 +| t7 +| s0 +| t16)
+      
+noextract
+let ws_next (#a:sha2_alg) (#m:m_spec)
+            (k:size_nat{k > 0 /\ k < v (num_rounds16 a)})
+            (ws:ws_spec a m) : ws_spec a m =
+    repeati 16 (ws_next_inner #a #m k) ws
+
+noextract
+let shuffle_inner (#a:sha2_alg) (#m:m_spec) (ws:ws_spec a m) (i:size_nat{i < v (num_rounds16 a)}) (j:size_nat{j < 16}) (st:state_spec a m) : state_spec a m =
+  let k_t = Seq.index (Spec.k0 a) (16 * i + j) in
+  let ws_t = ws.[j] in
+  shuffle_core_spec k_t ws_t st
+  
+noextract
+let shuffle_inner_loop (#a:sha2_alg) (#m:m_spec) (i:size_nat{i < v (num_rounds16 a)})
+                       (ws_st:ws_spec a m & state_spec a m) : ws_spec a m & state_spec a m =
+  let (ws,st) = ws_st in
+  let st' = repeati 16 (shuffle_inner ws i) st in
+  let ws' = if i < v (num_rounds16 a) - 1 then ws_next (i+1) ws else ws in
+  (ws',st')
+
+noextract
+let shuffle (#a:sha2_alg) (#m:m_spec) (ws:ws_spec a m) (st:state_spec a m) : state_spec a m =
+  let (ws,st) = repeati (v(num_rounds16 a)) (shuffle_inner_loop #a #m) (ws,st) in
+  st
+
+noextract
+let init (#a:sha2_alg) (#m:m_spec) : state_spec a m =
+  createi 8 (fun i -> load_element a m (Seq.index (Spec.h0 a) i))
+
+noextract
+let update (#a:sha2_alg) (#m:m_spec) (b:multiblock_spec a m) (st:state_spec a m): state_spec a m =
+  let st_old = st in
+  let ws = load_ws b in
+  let st_new = shuffle ws st_old in
+  map2 (+|) st_new st_old
+
+noextract
+let padded_blocks (a:sha2_alg) (len:size_nat{len < block_length a}) : n:nat{n <= 2} =
+  if (len + len_length a + 1 <= block_length a) then 1 else 2
+
+noextract
+let load_last1 (#a:sha2_alg) (#m:m_spec{lanes a m == 1}) (totlen:len_t a)
+               (len:size_nat{len < block_length a}) (b:multiseq 1 len) :
+               multiseq 1 (block_length a) & multiseq 1 (block_length a) & blocks:nat{blocks <= 2} =
+    let last = create (2 * block_length a) (u8 0) in
+    let last = update_sub last 0 len b in
+    let last = last.[len] <- u8 0x80 in
+    let total_len_bits = secret (shift_left #(len_int_type a) totlen 3ul) in 
+    let blocks = padded_blocks a len in
+    let fin = blocks * block_length a in
+    let len_by = Lib.ByteSequence.uint_to_bytes_be #(len_int_type a) total_len_bits in
+    let last = update_sub last (fin - len_length a) (len_length a) len_by in
+    let b0 = sub last 0 (block_length a) in
+    let b1 = sub last (block_length a) (block_length a) in
+    (b0, b1,blocks)
+
+#push-options "--z3rlimit 200"
+noextract
+let load_last4 (#a:sha2_alg) (#m:m_spec{lanes a m == 4}) (totlen:len_t a)
+               (len:size_nat{len < block_length a}) (b:multiseq 4 len) :
+               multiseq 4 (block_length a) & multiseq 4 (block_length a) & blocks:nat{blocks <= 2} =
+    let last = create (4 * 2 * block_length a) (u8 0) in
+    let last0 = sub last 0 (2 * block_length a) in
+    let last1 = sub last (2 * block_length a) (2 * block_length a) in
+    let last2 = sub last (4 * block_length a) (2 * block_length a) in
+    let last3 = sub last (6 * block_length a) (2 * block_length a) in
+    let last0 = update_sub last0 0 len b.(|0|) in
+    let last1 = update_sub last1 0 len b.(|1|) in
+    let last2 = update_sub last2 0 len b.(|2|) in
+    let last3 = update_sub last3 0 len b.(|3|) in
+    let last0 = last0.[len] <- u8 0x80 in
+    let last1 = last1.[len] <- u8 0x80 in
+    let last2 = last2.[len] <- u8 0x80 in
+    let last3 = last3.[len] <- u8 0x80 in
+    let total_len_bits = secret (shift_left #(len_int_type a) totlen 3ul) in 
+    let blocks = padded_blocks a len in
+    let fin = blocks * block_length a in
+    let len_by = Lib.ByteSequence.uint_to_bytes_be #(len_int_type a) total_len_bits in
+    let last0 = update_sub last0 (fin - len_length a) (len_length a) len_by in
+    let last1 = update_sub last1 (fin - len_length a) (len_length a) len_by in
+    let last2 = update_sub last2 (fin - len_length a) (len_length a) len_by in
+    let last3 = update_sub last3 (fin - len_length a) (len_length a) len_by in
+    let l00 = sub last0 0 (block_length a) in
+    let l10 = sub last1 0 (block_length a) in
+    let l20 = sub last2 0 (block_length a) in
+    let l30 = sub last3 0 (block_length a) in
+    let l01 = sub last0 (block_length a) (block_length a) in
+    let l11 = sub last1 (block_length a) (block_length a) in
+    let l21 = sub last2 (block_length a) (block_length a) in
+    let l31 = sub last3 (block_length a) (block_length a) in
+    let mb0:multiseq 4 (block_length a) = (l00, (l10, (l20, l30))) in
+    let mb1:multiseq 4 (block_length a) = (l01, (l11, (l21, l31))) in
+    (mb0,mb1,blocks)
+#pop-options
+
+noextract
+let load_last (#a:sha2_alg) (#m:m_spec) (totlen:len_t a)
+              (len:size_nat{len < block_length a}) (b:multiseq (lanes a m) len) :
+              multiseq (lanes a m) (block_length a) & multiseq (lanes a m) (block_length a) & blocks:nat{blocks <= 2} =
+    match lanes a m with
+    | 1 -> let (b0,b1,blocks) = load_last1 #a #m totlen len b  in
+           (b0,b1,blocks)
+    | 4 -> let mb: multiseq 4 len = tup4 b in
+           load_last4 #a #m totlen len mb
+    | _ -> admit()
+
+noextract
+let update_last (#a:sha2_alg) (#m:m_spec) (totlen:len_t a)
+                (len:size_nat{len < block_length a})
+                (b:multiseq (lanes a m) len) (st:state_spec a m): state_spec a m =
+  let (b0,b1,blocks) = load_last #a #m totlen len b in
+  let st = update b0 st in
+  if blocks > 1 then
+    update b1 st
+  else st
+
+noextract
+let transpose_hash1 (#a:sha2_alg) (#m:m_spec{lanes a m == 1})
+                    (st:state_spec a m) : state_spec a m = st
+
+noextract
+let transpose_hash4 (#a:sha2_alg) (#m:m_spec{lanes a m == 4})
+                    (st:state_spec a m) : state_spec a m =
+    let st0 = st.[0] in
+    let st1 = st.[1] in
+    let st2 = st.[2] in
+    let st3 = st.[3] in
+    let st4 = st.[4] in
+    let st5 = st.[5] in
+    let st6 = st.[6] in
+    let st7 = st.[7] in
+    let (st0,st1,st2,st3) = transpose4x4 (st0,st1,st2,st3) in
+    let (st4,st5,st6,st7) = transpose4x4 (st4,st5,st6,st7) in
+    create8 st0 st1 st2 st3 st4 st5 st6 st7 
+
+noextract
+let finish1 (#a:sha2_alg) (#m:m_spec{lanes a m == 1})
+           (st:state_spec a m) : multiseq (lanes a m) (hash_length a) =
+    let st = transpose_hash1 st in
+    let h = create (8 * word_length a) (u8 0) in
+    let h = repeati 8 (fun i h -> 
+                    update_sub h (i * word_length a) (word_length a)
+                      (vec_to_bytes_be st.[i])) h in
+    let hsub = sub h 0 (hash_length a) in
+    hsub <: multiseq 1 (hash_length a)
+
+#push-options "--z3rlimit 100"
+noextract
+let finish4 (#a:sha2_alg) (#m:m_spec{lanes a m == 4})
+           (st:state_spec a m) : multiseq 4 (hash_length a) =
+    let st = transpose_hash4 st in
+    let h = create (8 * 4 * word_length a) (u8 0) in
+    let h = repeati 8 (fun i h -> 
+                    update_sub h (i * 4 * word_length a) (4 * word_length a)
+                      (vec_to_bytes_be st.[i])) h in
+    let h0 = sub h 0 (8 * word_length a) in
+    let h1 = sub h (8 * word_length a) (8 * word_length a) in
+    let h2 = sub h (16 * word_length a) (8 * word_length a) in
+    let h3 = sub h (24 * word_length a) (8 * word_length a) in
+    let hsub0 : lseq uint8 (hash_length a) = sub h0 0 (hash_length a) in
+    let hsub1 : lseq uint8 (hash_length a) = sub h1 0 (hash_length a) in
+    let hsub2 : lseq uint8 (hash_length a) = sub h2 0 (hash_length a) in
+    let hsub3 : lseq uint8 (hash_length a) = sub h3 0 (hash_length a) in
+    let hsub : multiseq 4 (hash_length a) = (hsub0,(hsub1,(hsub2,hsub3))) in
+    hsub <: multiseq 4 (hash_length a)
+#pop-options
+
+noextract
+let finish (#a:sha2_alg) (#m:m_spec)
+           (st:state_spec a m) : multiseq (lanes a m) (hash_length a) =
+    match lanes a m with
+    | 1 -> finish1 st
+    | 4 -> finish4 st
+    | _ -> admit()
+
+#push-options "--z3rlimit 200 --max_ifuel 2 --max_fuel 2"
+noextract
+let get_multiblock_spec (#a:sha2_alg) (#m:m_spec)
+                        (len:size_nat) (b:multiseq (lanes a m) len)
+                        (i:size_nat{i < len / block_length a})
+                        : multiseq (lanes a m) (block_length a) =
+    match lanes a m with
+    | 1 -> let r = sub #_ #len  (b <: multiseq 1 len) (i * block_length a) (block_length a) in
+           r <: multiseq 1 (block_length a)
+    | 4 -> let (b0,(b1,(b2,b3))) = tup4 b in
+           let bl0 = sub (b0 <: lseq uint8 len) (i * block_length a) (block_length a) in
+           let bl1 = sub (b1 <: lseq uint8 len) (i * block_length a) (block_length a) in
+           let bl2 = sub (b2 <: lseq uint8 len) (i * block_length a) (block_length a) in
+           let bl3 = sub (b3 <: lseq uint8 len) (i * block_length a) (block_length a) in
+           let ms: multiseq 4 (block_length a) = (bl0,(bl1,(bl2,bl3))) in
+           ms <: multiseq 4 (block_length a)
+    | _ -> admit()
+
+noextract
+let get_multilast_spec (#a:sha2_alg) (#m:m_spec)
+                        (len:size_nat) (b:multiseq (lanes a m) len)
+                        : multiseq (lanes a m) (len % block_length a) =
+    let rem = len % block_length a in
+    match lanes a m with
+    | 1 -> let r = sub #_ #len  (b <: multiseq 1 len) (len - rem) (rem) in
+           r <: multiseq 1 rem
+    | 4 -> let (b0,(b1,(b2,b3))) = tup4 b in
+           let bl0 = sub (b0 <: lseq uint8 len) (len - rem) rem in
+           let bl1 = sub (b1 <: lseq uint8 len) (len - rem) rem in
+           let bl2 = sub (b2 <: lseq uint8 len) (len - rem) rem in
+           let bl3 = sub (b3 <: lseq uint8 len) (len - rem) rem in
+           let ms: multiseq 4 rem = (bl0,(bl1,(bl2,bl3))) in
+           ms <: multiseq 4 rem
+    | _ -> admit()
+#pop-options                       
+
+noextract
+let hash (#a:sha2_alg) (#m:m_spec) (len:len_t a{len_v a len <= max_size_t}) (b:multiseq (lanes a m) (len_v a len)) =
+    let ls = len_v a len in
+    let st = init #a #m in
+    let blocks = ls / block_length a in
+    let rem = ls % block_length a in
+    let st = repeati blocks (fun i st ->
+      let mb = get_multiblock_spec ls b i in
+      update mb st) st in
+    let mb = get_multilast_spec #a #m ls b in
+    let st = update_last len rem mb st in
+    finish st
+
+noextract
+let sha256 (len:size_nat) (b:lseq uint8 len) =
+  hash #SHA2_256 #M32 (mk_int #U64 #PUB len) b
+
+noextract
+let sha256_4 (len:size_nat) (b:multiseq 4 len) =
+  hash #SHA2_256 #M128 (mk_int #U64 #PUB len) b
+
+noextract
+let sha512 (len:size_nat) (b:lseq uint8 len) =
+  hash #SHA2_512 #M32 (mk_int #U128 #PUB len) b
+
+noextract
+  let sha512_4 (len:size_nat) (b:multiseq 4 len) =
+  hash #SHA2_512 #M256 (mk_int #U128 #PUB len) b
